

# Discrete Mathematics Homework 5

1. Find the recurrence relation of  $D_n = \begin{vmatrix} a+b & ab & 0 & \cdots & 0 \\ 1 & a+b & ab & \ddots & \vdots \\ 0 & 1 & \ddots & \ddots & 0 \\ \vdots & \ddots & \ddots & a+b & ab \\ 0 & \cdots & 0 & 1 & a+b \end{vmatrix}_{n \times n}$ . Hence calculate  $D_n$ .

Solution

Expand along the first row, we have

$$D_n = \begin{vmatrix} a+b & ab & 0 & \cdots & 0 \\ 1 & a+b & ab & \ddots & \vdots \\ 0 & 1 & \ddots & \ddots & 0 \\ \vdots & \ddots & \ddots & a+b & ab \\ 0 & \cdots & 0 & 1 & a+b \end{vmatrix}_{n \times n}$$

$$= (a+b) \begin{vmatrix} a+b & ab & 0 & \cdots & 0 \\ 1 & a+b & ab & \ddots & \vdots \\ 0 & 1 & \ddots & \ddots & 0 \\ \vdots & \ddots & \ddots & a+b & ab \\ 0 & \cdots & 0 & 1 & a+b \end{vmatrix}_{(n-1) \times (n-1)} - ab \begin{vmatrix} 1 & ab & 0 & \cdots & 0 \\ 0 & a+b & ab & \ddots & \vdots \\ 0 & 1 & \ddots & \ddots & 0 \\ \vdots & \ddots & \ddots & a+b & ab \\ 0 & \cdots & 0 & 1 & a+b \end{vmatrix}_{(n-1) \times (n-1)}$$

$$= (a+b)D_{n-1} - abD_{n-2}$$

We now obtain the relation  $D_n - (a+b)D_{n-1} + abD_{n-2} = 0, n \geq 3$  with

$$D_1 = a+b, D_2 = \begin{vmatrix} a+b & ab \\ 1 & a+b \end{vmatrix} = (a+b)^2 - ab = a^2 + ab + b^2.$$

The characteristic equation  $r^2 - (a+b)r + ab = 0$  has roots  $a$  and  $b$ .

Case (i): one of  $a, b = 0$

Suppose  $b = 0$ .

$$D_n = aD_{n-1} = a^{n-1}D_1 = a^n.$$

Case (ii):  $a \neq b, a, b \neq 0$ .

$$\begin{matrix} a=b=0 & 1 \\ a=0 & b \neq 0 & 1 \\ a \neq 0 & b=0 & 1 \end{matrix}$$

$$D_n = c_1 a^n + c_2 b^n$$

$$D_1 = a + b = c_1 a + c_2 b,$$

$$D_2 = a^2 + ab + b^2 = c_1 a^2 + c_2 b^2$$

$$\begin{pmatrix} a & b \\ a^2 & b^2 \end{pmatrix} \begin{pmatrix} c_1 \\ c_2 \end{pmatrix} = \begin{pmatrix} a+b \\ a^2+ab+b^2 \end{pmatrix} \quad \}$$

$$\begin{pmatrix} c_1 \\ c_2 \end{pmatrix} = \frac{1}{ab^2 - ba^2} \begin{pmatrix} b^2 & -b \\ -a^2 & a \end{pmatrix} \begin{pmatrix} a+b \\ a^2+ab+b^2 \end{pmatrix}$$

$$= \frac{1}{ab^2 - ba^2} \begin{pmatrix} b^2(a+b) - b(a^2 + ab + b^2) \\ -a^2(a+b) + a(a^2 + ab + b^2) \end{pmatrix}$$

$$= \frac{1}{ab^2 - ba^2} \begin{pmatrix} -ba^2 \\ ab^2 \end{pmatrix}$$

$$= \frac{1}{b-a} \begin{pmatrix} -a \\ b \end{pmatrix}$$

$$D_n = \frac{b^{n+1} - a^{n+1}}{b-a}$$

Case (iii):  $a = b \neq 0$ .

$$D_n = (c_1 + c_2 n) a^n \quad \text{4}$$

$$D_1 = 2a = (c_1 + c_2) a,$$

$$D_2 = 3a^2 = (c_1 + 2c_2) a^2$$

$$c_1 = c_2 = 1$$

$$D_n = (1+n) a^n$$

2. Solve each of the following recurrence relations. 20

(a)  $a_{n+2} + 3a_{n+1} + 2a_n = 3^n, \quad n \geq 0, \quad a_0 = 0, \quad a_1 = 1.$  4

(b)  $a_{n+2} + 4a_{n+1} + 4a_n = 7, \quad n \geq 0, \quad a_0 = 1, \quad a_1 = 2.$  4

(c)  $a_{n+2}^2 - 5a_{n+1}^2 + 6a_n^2 = 7n, \quad n \geq 0, \quad a_0 = 1, \quad a_1 = 1.$  4

(d)  $a_{n+1} - 2a_n = 2^n, \quad n \geq 0, \quad a_0 = 1.$  4

(e)  $a_n + 2a_{n-1} + 2a_{n-2} = 0, \quad n \geq 2, \quad a_0 = 1, \quad a_1 = 3.$  4

Solution

→ 10

explain 2  
answer 2

(a)  $a_{n+2} + 3a_{n+1} + 2a_n = 3^n, n \geq 0, a_0 = 0, a_1 = 1.$

With  $a_n = cr^n, c, r \neq 0$ , the characteristic equation  $r^2 + 3r + 2 = 0 = (r+2)(r+1)$  yields the characteristic roots  $r = -1, -2$ .

Hence  $a_n^{(h)} = A(-1)^n + B(-2)^n$ , while  $a_n^{(p)} = C(3)^n$ .

$$C(3)^{n+2} + 3C(3)^{n+1} + 2C(3)^n = 3^n \implies 9C + 9C + 2C = 1 \implies C = 1/20.$$

$$a_n = A(-1)^n + B(-2)^n + (1/20)(3)^n$$

$$0 = a_0 = A + B + (1/20)$$

$$1 = a_1 = -A - 2B + (3/20)$$

Hence  $1 = a_0 + a_1 = -B + (4/20)$  and  $B = -4/5$ . Then  $A = -B - (1/20) = 3/4$ .

$$a_n = (3/4)(-1)^n + (-4/5)(-2)^n + (1/20)(3)^n, n \geq 0$$

(b)  $a_n = (2/9)(-2)^n - (5/6)(n)(-2)^n + (7/9), n \geq 0$

(c) Let  $a_n^2 = b_n, n \geq 0$

$$b_{n+2} - 5b_{n+1} + 6b_n = 7n$$

$$b_n^{(h)} = A(3^n) + B(2^n), b_n^{(p)} = Cn + D$$

$$C(n+2) + D - 5[C(n+1) + D] + 6(Cn + D) = 7n \implies C = 7/2, D = 21/4$$

$$b_n = A(3^n) + B(2^n) + (7n/2) + (21/4)$$

$$b_0 = a_0^2 = 1, b_1 = a_1^2 = 1$$

$$1 = b_0 = A + B + 21/4$$

$$1 = b_1 = 3A + 2B + 7/2 + 21/4$$

$$3A + 2B = -31/3$$

$$2A + 2B = -34/4$$

$$A = 3/4, B = -5$$

$$a_n = [(3/4)(3)^n - 5(2)^n + (7n/2) + (21/4)]^{1/2}, n \geq 0$$

(d)  $a_n = 2^n + n(2^{n-1}), n \geq 0.$

(e)  $a_n + 2a_{n-1} + 2a_{n-2} = 0, n \geq 2, a_0 = 1, a_1 = 3.$

$$r^2 + 2r + 2 = 0, r = -1 \pm i$$

$$(-1 + i) = \sqrt{2}(\cos(3\pi/4) + i \sin(3\pi/4))$$

$$(-1 - i) = \sqrt{2}(\cos(5\pi/4) + i \sin(5\pi/4)) =$$

$$\sqrt{2}(\cos(-3\pi/4) + i \sin(-3\pi/4)) = \sqrt{2}(\cos(3\pi/4) - i \sin(3\pi/4))$$

$$a_n = (\sqrt{2})^n [A \cos(3\pi n/4) + B \sin(3\pi n/4)]$$

$$1 = a_0 = A$$

$$3 = a_1 = \sqrt{2}[\cos(3\pi/4) + B \sin(3\pi/4)] =$$

$$\sqrt{2}[(-1/\sqrt{2}) + B(1/\sqrt{2})], \text{ so } 3 = -1 + B, B = 4$$

$$a_n = (\sqrt{2})^n [\cos(3\pi n/4) + 4 \sin(3\pi n/4)], n \geq 0$$

$$\frac{(-i)^n}{2} (-1+i)^n + \frac{(1+i)^n}{2} (-1-i)^n$$

3. Let  $a_n$  be the number of expression (not answer) of  $\underbrace{1-1-\dots-1-1}_n$  together with ( ) for each subtraction. For instance,

$$a_0 = 1:$$

$$1$$

$$a_1 = 1:$$

$$1 \ominus 1$$

$$a_2 = 2:$$

$$(1-1) \ominus 1, 1 \ominus (1-1)$$

$$a_3 = 5: ((1-1)-1) \ominus 1, (1-(1-1)) \ominus 1, (1-1)-(1-1), 1-((1-1)-1), 1-(1-(1-1))$$

(a) List all possible cases for  $n = 4$ .

7 (0.5 each)

(b) Find the recurrence relation for  $a_n$ . Explain your relation in detail.

6

(c) Hence, solve the  $a_n$ .

7

Solution

$$(a) a_4 = 14$$

$$1-(((1-1)-1)-1), 1-((1-(1-1))-1), 1-((1-1)-(1-1)), 1-(1-((1-1)-1)), 1-(1-(1-(1-1)))$$

$$(1-1)-((1-1)-1), (1-1)-(1-(1-1))$$

$$((1-1)-1)-(1-1), (1-(1-1))-(1-1)$$

$$(((1-1)-1)-1)-1, (((1-(1-1))-1)-1), ((1-1)-(1-1))-1, (1-((1-1)-1))-1, (1-(1-(1-1)))-1$$

$$(b) \underbrace{1-1-\dots-1-1}_n = \underbrace{\left( \underbrace{1-1-\dots-1-1}_k \right)}_{\text{main subtraction}} \ominus \underbrace{\left( \underbrace{1-1-\dots-1-1}_{n-k-1} \right)}_{\text{"-"}} , \quad 0 \leq k \leq n-1$$

$$\underbrace{\left( \underbrace{1-1-\dots-1-1}_k \right)}_{\text{"-"}} \text{ has } a_k \text{ choices, } \underbrace{\left( \underbrace{1-1-\dots-1-1}_{n-k-1} \right)}_{\text{"-"}} \text{ has } a_{n-k-1} \text{ choices.}$$

$$a_n = a_0 a_{n-1} + a_1 a_{n-2} + \dots + a_{n-1} a_0, \quad n \geq 1.$$

(c) Let  $f(x) = \sum_{n=0}^{\infty} a_n x^n$  be the generating functions of  $a_n$ . Multiplying  $x^n$  to above equation, we obtain

$$a_n x^n = x \left( a_0 a_{n-1} x^{n-1} + a_1 a_{n-2} x^{n-2} + \dots + a_{n-1} x^{n-1} a_0 \right), \quad n \geq 1.$$

$$\sum_{n=1}^{\infty} a_n x^n = x \left( \sum_{n=0}^{\infty} a_n x^n \right)^2$$

$$f(x) - a_0 = x f(x)^2$$

$$f(x) = 1 + x f(x)^2$$

$$x f(x)^2 - f(x) + 1 = 0$$

Recall  $\binom{\frac{1}{2}}{n} = \frac{(\frac{1}{2})(\frac{1}{2}-1)\cdots(\frac{1}{2}-n+1)}{n!} = \frac{(-1)^{n-1}}{2^n} \cdot \frac{1 \cdot 3 \cdots (2n-3)}{n!} = (-1)^{n-1} \left(\frac{1}{2}\right)^{2n-1} \frac{(2n-2)!}{n!(n-1)!}, \quad n \geq 1.$

Then

$$(1-x)^{\frac{1}{2}} = \binom{\frac{1}{2}}{0} + \binom{\frac{1}{2}}{1}(-x) + \cdots + \binom{\frac{1}{2}}{n}(-x)^n + \cdots = 1 - \frac{1}{2}x - \cdots - \left(\frac{1}{2}\right)^{2n-1} \frac{(2n-2)!}{n!(n-1)!} x^n - \cdots.$$

$$f(x) = \frac{1 - \sqrt{1-4x}}{2x}$$

$$= \frac{1}{2x} \left( 1 - \left( 1 - \frac{1}{2}(4x) - \cdots - \left(\frac{1}{2}\right)^{2n-1} \frac{(2n-2)!}{n!(n-1)!} (4x)^n - \cdots \right) \right)$$

explain: f

$$= \frac{1}{2x} \left( \frac{1}{2}(4x) + \cdots + \left(\frac{1}{2}\right)^{2n-1} \frac{(2n-2)!}{n!(n-1)!} 2^{2n} x^n + \cdots \right)$$

$$= \frac{1}{2x} \left( \frac{1}{2}(4x) + \cdots + \frac{(2n-2)!}{n!(n-1)!} 2x^n + \cdots \right)$$

$$= 1 + \cdots + \frac{(2n-2)!}{n!(n-1)!} x^{n-1} + \cdots$$

$$a_n = \frac{(2n)!}{n!(n+1)!}$$

✓

4. Solve the systems of recurrence relation

$$a_{n+1} = -2a_n - 4b_n$$

$$b_{n+1} = 4a_n + 6b_n$$

$$n \geq 0, a_0 = 1, b_0 = 0$$

20

Solution

$$a_{n+2} = -2a_{n+1} - 4b_{n+1}$$

$$a_0 = 1$$

$$= 4a_n + 8b_n - 16a_n - 24b_n$$

$$a_1 = -2$$

$$= -12a_n - 16b_n$$

②

②

$$a_{n+2} - 4a_{n+1} = 4a_n$$

$$C_1 2^n + C_2 n 2^n$$

$$a_{n+1} = -2a_n - 4b_n$$

$$b_{n+1} = 4a_n + 6b_n$$

$$n \geq 0, a_0 = 1, b_0 = 0.$$

$$\text{Let } f(x) = \sum_{n=0}^{\infty} a_n x^n, g(x) = \sum_{n=0}^{\infty} b_n x^n.$$

$$\sum_{n=0}^{\infty} a_{n+1} x^{n+1} = -2 \sum_{n=0}^{\infty} a_n x^{n+1} - 4 \sum_{n=0}^{\infty} b_n x^{n+1}$$

$$\sum_{n=0}^{\infty} b_{n+1} x^{n+1} = 4 \sum_{n=0}^{\infty} a_n x^{n+1} + 6 \sum_{n=0}^{\infty} b_n x^{n+1}$$

$$f(x) - a_0 = -2xf(x) - 4xg(x)$$

$$g(x) - b_0 = 4xf(x) + 6xg(x)$$

$$f(x)(1 + 2x) + 4xg(x) = 1$$

$$f(x)(-4x) + (1 - 6x)g(x) = 0$$

$$f(x) = \frac{\begin{vmatrix} 1 & 4 \\ 0 & (1-6x) \end{vmatrix}}{\begin{vmatrix} (1+2x) & 4x \\ -4x & (1-6x) \end{vmatrix}} = (1-6x)/(1-2x)^2 =$$

$$(1-6x)(1-2x)^{-2} = (1-6x)[\binom{-2}{0} + \binom{-2}{1}(-2x) + \binom{-2}{2}(-2x)^2 + \dots]$$

$$a_n = \binom{-2}{n}(-2)^n - 6\binom{-2}{n-1}(-2)^{n-1} = 2^n(1-2n), n \geq 0$$

$$f(x)(-4x) + (1-6x)g(x) = 0 \implies g(x) = (4x)f(x)(1-6x)^{-1} \implies g(x) = 4x(1-2x)^{-2} \text{ and } b_n = 4\binom{-2}{n-1}(-2)^{n-1} = n(2^{n+1}), n \geq 0.$$

3. Find the recurrence relation of  $D_n = \begin{vmatrix} 0 & 1 & 1 & 1 & \dots & 1 \\ 1 & 0 & 1 & 1 & \dots & 1 \\ 1 & 1 & 0 & 1 & \dots & 1 \\ \vdots & \vdots & \ddots & \ddots & \ddots & \vdots \\ 1 & \vdots & \dots & 1 & 0 & 1 \\ 1 & 1 & \dots & 1 & 1 & 0 \end{vmatrix}_{n \times n}$ . Hence calculate  $D_n$ .

Hint:  $C_1 - C_n \rightarrow C_1$ .

Solution

$$\begin{aligned}
& \begin{vmatrix} 0 & 1 & 1 & 1 & \cdots & 1 \\ 1 & 0 & 1 & 1 & \cdots & 1 \\ 1 & 1 & 0 & 1 & \cdots & 1 \\ \vdots & \vdots & \ddots & \ddots & \ddots & \vdots \\ 1 & \vdots & \cdots & 1 & 0 & 1 \\ 1 & 1 & \cdots & 1 & 1 & 0 \end{vmatrix}_{n \times n} = \begin{vmatrix} -1 & 1 & 1 & 1 & \cdots & 1 \\ 0 & 0 & 1 & 1 & \cdots & 1 \\ 0 & 1 & 0 & 1 & \cdots & 1 \\ \vdots & \vdots & \ddots & \ddots & \ddots & \vdots \\ 0 & \vdots & \cdots & 1 & 0 & 1 \\ 1 & 1 & \cdots & 1 & 1 & 0 \end{vmatrix}_{n \times n} \quad [C_1 - C_n \rightarrow C_1] \\
& = \begin{vmatrix} -2 & 0 & 0 & \cdots & 0 & 1 \\ 0 & 0 & 1 & 1 & \cdots & 1 \\ 0 & 1 & 0 & 1 & \cdots & 1 \\ \vdots & \vdots & \ddots & \ddots & \ddots & \vdots \\ 0 & \vdots & \cdots & 1 & 0 & 1 \\ 1 & 1 & \cdots & 1 & 1 & 0 \end{vmatrix}_{n \times n} \quad [R_1 - R_n \rightarrow R_1] \\
& = -2 \begin{vmatrix} 0 & 1 & 1 & \cdots & 1 \\ 1 & 0 & 1 & \cdots & 1 \\ \vdots & \ddots & \ddots & \ddots & \vdots \\ \vdots & \cdots & 1 & 0 & 1 \\ 1 & \cdots & 1 & 1 & 0 \end{vmatrix}_{(n-1) \times (n-1)} + (-1)^{1+n} \begin{vmatrix} 0 & 0 & \cdots & 0 & 1 \\ 0 & 1 & 1 & \cdots & 1 \\ 1 & 0 & 1 & \cdots & 1 \\ \vdots & \ddots & \ddots & \ddots & \vdots \\ 1 & \cdots & 1 & 0 & 1 \end{vmatrix}_{(n-1) \times (n-1)} \\
& = -2 \begin{vmatrix} 0 & 1 & 1 & \cdots & 1 \\ 1 & 0 & 1 & \cdots & 1 \\ \vdots & \ddots & \ddots & \ddots & \vdots \\ \vdots & \cdots & 1 & 0 & 1 \\ 1 & \cdots & 1 & 1 & 0 \end{vmatrix}_{(n-1) \times (n-1)} + (-1)^{1+n} (-1)^{1+n-1} \begin{vmatrix} 0 & 1 & \cdots & 1 \\ 1 & 0 & \ddots & \vdots \\ \vdots & \ddots & \ddots & 1 \\ 1 & \cdots & 1 & 0 \end{vmatrix}_{(n-2) \times (n-2)}
\end{aligned}$$

$$D_n + 2D_{n-1} + D_{n-2} = 0 \quad \Rightarrow \quad 8 \text{ explain}$$

$$D_n = (-1)^n (A + Bn)$$

$$(-1)(A + B) = D_1 = 0, \quad (A + 2B) = D_2 = -1$$

$$B = -1, \quad A = 1$$

$$D_n = (-1)^n (1 - n)$$

10

$$\begin{vmatrix} 0 & 1 & \dots & 1 \\ 1 & 0 & \dots & 1 \\ \vdots & \vdots & \ddots & \vdots \\ 1 & 1 & \dots & 0 \end{vmatrix}_{n \times n} \quad \underline{\underline{C_i = C_i - C_n}} \quad \begin{vmatrix} -1 & 1 & \dots & 1 \\ 0 & 0 & \dots & 1 \\ \vdots & \vdots & \ddots & \vdots \\ 1 & 1 & \dots & 0 \end{vmatrix}_{n \times n}$$

$$= (-1)^{1+n} (-1) \begin{vmatrix} 0 & 1 & \dots & 1 \\ 1 & 0 & \dots & 1 \\ \vdots & \vdots & \ddots & \vdots \\ 1 & 1 & \dots & 0 \end{vmatrix}_{(n-1) \times (n-1)}$$

$$+ (-1)^{n+1} \cdot 1 \cdot \begin{vmatrix} 1 & 1 & \dots & 1 \\ 0 & 1 & \dots & 1 \\ \vdots & \vdots & \ddots & \vdots \\ 1 & 1 & \dots & 0 \end{vmatrix}_{(n-1) \times (n-1)}$$

$$= -D_{n-1} + (-1)^{n+1} \begin{vmatrix} 1 & 1 & \dots & 1 \\ 0 & 1 & \dots & 1 \\ \vdots & \vdots & \ddots & \vdots \\ 1 & 1 & \dots & 0 \end{vmatrix}_{(n-1) \times (n-1)}$$

$$D_n = -D_{n-1} + (-1)^{n+1}$$

$$\begin{aligned} R_2 &= R_2 - R_1 \\ &\vdots \\ R_{n-1} &= R_{n-1} - R_1 \\ &= (-1)^n (-1)^{n-2} \\ &= 1 \end{aligned} \quad \begin{vmatrix} 1 & 1 & \dots & 1 \\ -1 & 0 & \dots & 0 \\ \vdots & \vdots & \ddots & \vdots \\ 0 & 0 & \dots & -1 \end{vmatrix}$$